some progress

advanced11.lean
@@ -2,12 +2,122 @@ import Mathlib.Tactic
 
 open Set
 open Finset
+open Nat
 
 -- x divides an odd number of elements of B
-def oddDivides (x : ℕ) (B : Finset ℕ) := ¬(card (B.filter (fun y ↦ x∣y)) ∣ 2)  
+def odd_divides (x : ℕ) (B : Finset ℕ) : Bool :=
+  card (B.filter (x ∣ ·)) % 2 ≠ 0
 
--- If A is a subset of a finite set X⊆ℤ⁺, then there exists a subset B⊆X such that A is the set of elements of X that divide an odd number of elements of B.
-theorem advanced11 (X A B: Finset ℕ) (h₁ : A ⊆ X) (h₂ : B ⊆ X) (z : 0∉X)
-  : ∃B,(A = {x∈X | oddDivides x B}) := by
+#eval (fun x B ↦ (filter (x ∣ ·) B).card % 2 ≠ 0) 2 { 1, 2, 3, 4 }
+#eval odd_divides 2 { 1, 2, 3, 4 }
+
+example : odd_divides 2 { 1, 2, 3 } := by
+  simp [odd_divides]
+  done
+
+example (i k : ℕ) (h : i ≤ k) : i - 1 ≤ k := by
+  { norm_num; exact Nat.le_step h }
+
+def calc_Xᵢ (i : ℕ) (X : Finset ℕ) : Finset ℕ :=
+  List.toFinset $ List.take i $ X.sort (· ≥ ·)
+
+lemma eq_calc_zero (X : Finset ℕ) : calc_Xᵢ 0 X = {} := by
+  simp [calc_Xᵢ]
+  done
+
+lemma list_take_subset (X : List ℕ) (k : ℕ)
+  : List.take k X ⊆ List.take (k + 1) X := by
+  intro x h
+  rw [List.take_succ]
+  simp only [List.mem_append, Option.mem_toList, Option.mem_def]
+  constructor
+  exact h
+  done
+
+lemma finset_subset (X Y: List ℕ) (h : X ⊆ Y)
+  : X.toFinset ⊆ Y.toFinset := by
+  intro x h2
+  simp at h2 ⊢
+  exact h h2
+  done
+
+lemma calc_X_inc (X : Finset ℕ) (i : ℕ)
+  : calc_Xᵢ i X ⊆ calc_Xᵢ (Nat.succ i) X := by
+  simp [calc_Xᵢ, list_take_subset, finset_subset]
+  done
+
+def calc_Aᵢ (i : ℕ) (X A : Finset ℕ) : Finset ℕ :=
+  A ∩ calc_Xᵢ i X
+
+def calc_Bᵢ (i : ℕ) (X A : Finset ℕ) : Finset ℕ := match i with
+  | 0 => ∅
+  | k + 1 =>
+    if h : X.card < k + 1 then calc_Bᵢ X.card X A else
+    let xₖ := (X.sort (· ≥ ·))[k]'(by simp at *; exact h)
+    let Bₖ := calc_Bᵢ k X A
+    let c := Or (And (xₖ ∈ A) (odd_divides xₖ Bₖ)) (And (xₖ ∉ A) ¬(odd_divides xₖ Bₖ))
+    Bₖ ∪ (if (¬ c) then { xₖ } else ∅)
+
+#eval calc_Xᵢ 3 { 1, 2, 3 }
+#eval calc_Aᵢ 1 { 1, 2, 3 } { 1, 2 }
+#eval calc_Aᵢ 2 { 1, 2, 3 } { 1, 2 }
+#eval calc_Aᵢ 3 { 1, 2, 3 } { 1, 2 }
+#eval calc_Bᵢ 1 { 1, 2, 3 } { 1, 2 }
+#eval calc_Bᵢ 2 { 1, 2, 3 } { 1, 2 }
+#eval calc_Bᵢ 3 { 1, 2, 3 } { 1, 2 }
+
+def adv_11_ith_step (X A B : Finset ℕ) (h₁ : A ⊆ X) (h₂ : B ⊆ X) (z : 0 ∉ X) (i : ℕ) :=
+  let Aᵢ := calc_Aᵢ i X A
+  let Bᵢ := calc_Bᵢ i X A
+  let Xᵢ := calc_Xᵢ i X
+  Aᵢ = { x ∈ Xᵢ | odd_divides x Bᵢ }
+
+def const_set (i: ℕ) : Finset ℕ := match i with
+  | 0 => { 0 }
+  | k + 1 => const_set (k) ∪ { i }
+
+lemma const_set_mono (i: ℕ) : const_set (i) ⊆ const_set (i + 1) := by
   sorry
+  done
+
+lemma calc_Bᵢ_mono (X A : Finset ℕ) (i : ℕ)
+  : calc_Bᵢ i X A ⊆ calc_Bᵢ (i + 1) X A := by
+  intro x hₓ
+  unfold calc_Bᵢ
+  split_ifs
+  · unfold calc_Bᵢ
+    split
+    . simp
+      unfold calc_Bᵢ at hₓ
+      split at hₓ
+      . contradiction
+      .
+    . sorry
+  . simp
+    apply Or.inl
+    exact hₓ
+  done
+
+lemma adv_11_base (X A B: Finset ℕ) (h₁ : A ⊆ X) (h₂ : B ⊆ X) (z : 0 ∉ X)
+      : adv_11_ith_step X A B h₁ h₂ z 0 := by
+  simp [adv_11_ith_step, calc_Aᵢ, eq_calc_zero, Finset.inter_empty]
+  done
+
+lemma adv_11_ind (X A B: Finset ℕ) (h₁ : A ⊆ X) (h₂ : B ⊆ X) (z : 0 ∉ X) (k : ℕ)
+    : adv_11_ith_step X A B h₁ h₂ z k → adv_11_ith_step X A B h₁ h₂ z (k + 1) := by
+  repeat rw [adv_11_ith_step]
+  intro hy
+  rw [Set.Subset.antisymm_iff]
+
+  constructor
+  . -- simp [calc_Aᵢ]
+    intro x hₓ
+    by_cases (x ∈ calc_Aᵢ k X A)
+    . have : x ∈ {x | x ∈ calc_Xᵢ k X ∧ odd_divides x B} := by { rw [← hy]; exact h }
+      have : x ∈ calc_Xᵢ k X ∧ odd_divides x B := this
+      constructor
+      . exact Finset.mem_of_mem_inter_right hₓ
+      . exact this.right
+    . sorry
+  . sorry
   done
